Semantics.v
@@ -1,4 +1,4 @@
-Require Import Coq.Lists.List.
+Require Import Coq.Lists.List Coq.Bool.Bool.
 Require Export SGA.Common SGA.Environments SGA.Syntax SGA.TypedSyntax.
 
 Import ListNotations.
@@ -55,6 +55,12 @@ Section Logs.
   Definition log_find {T} (log: Log) reg (f: @LogEntry (R reg) -> option T) : option T :=
     list_find_opt f (REnv.(getenv) log reg).
 
+  Lemma log_find_empty {T} idx (f: @LogEntry (R idx) -> option T):
+    log_find (log_empty: Log) idx f = None.
+  Proof.
+    unfold log_find, log_empty; intros; rewrite getenv_create; reflexivity.
+  Qed.
+
   Lemma log_find_app {T} (l l': Log) reg (f: @LogEntry (R reg) -> option T) :
     log_find (log_app l l') reg f =
     match log_find l reg f with
@@ -68,11 +74,147 @@ Section Logs.
     reflexivity.
   Qed.
 
+  Definition log_cons (reg: reg_t) le (l: Log) :=
+    REnv.(putenv) l reg (le :: REnv.(getenv) l reg).
+
+  Lemma log_cons_eq :
+    forall (log: Log) idx le,
+      REnv.(getenv) (log_cons idx le log) idx = le :: REnv.(getenv) log idx.
+  Proof.
+    unfold log_cons; intros; rewrite get_put_eq; reflexivity.
+  Qed.
+
+  Lemma log_cons_neq :
+    forall (log: Log) idx idx' le,
+      idx <> idx' ->
+      REnv.(getenv) (log_cons idx' le log) idx = REnv.(getenv) log idx.
+  Proof.
+    unfold log_cons; intros; rewrite get_put_neq; eauto.
+  Qed.
+
+  Lemma log_find_cons_eq {T}:
+    forall (log: Log) idx le (f: _ -> option T),
+      log_find (log_cons idx le log) idx f =
+      match f le with
+      | Some v => Some v
+      | _ => log_find log idx f
+      end.
+  Proof.
+    unfold log_find; intros;
+      rewrite log_cons_eq; reflexivity.
+  Qed.
+
+  Lemma log_find_cons_neq {T}:
+    forall (log: Log) idx idx' le (f: _ -> option T),
+      idx <> idx' ->
+      log_find (log_cons idx' le log) idx f =
+      log_find log idx f.
+  Proof.
+    unfold log_find; intros;
+      rewrite log_cons_neq by eassumption; reflexivity.
+  Qed.
+
   Definition log_forallb (log: Log) reg (f: LogEntryKind -> Port -> bool) :=
     List.forallb (fun '(LE _ kind prt _) => f kind prt) (REnv.(getenv) log reg).
 
-  Definition log_cons (reg: reg_t) le (l: Log) :=
-    REnv.(putenv) l reg (le :: REnv.(getenv) l reg).
+  Definition log_existsb (log: Log) reg (f: LogEntryKind -> Port -> bool) :=
+    List.existsb (fun '(LE _ kind prt _) => f kind prt) (REnv.(getenv) log reg).
+
+  (* FIXME move these lemmas out of the semantics *)
+  Lemma log_forallb_not_existb (log: Log) reg (f: LogEntryKind -> Port -> bool) :
+    negb (log_existsb log reg f) = log_forallb log reg (fun k p => negb (f k p)).
+  Proof.
+    unfold log_existsb, log_forallb.
+    induction (getenv _ _ _); cbn.
+    - reflexivity.
+    - destruct a; cbn.
+      rewrite negb_orb, IHy.
+      reflexivity.
+  Qed.
+
+  Lemma log_existsb_log_cons_eq :
+    forall (log: Log) idx k p v f,
+      log_existsb (log_cons idx (LE _ k p v) log) idx f =
+      f k p || log_existsb log idx f.
+  Proof.
+    unfold log_existsb; intros; rewrite log_cons_eq; reflexivity.
+  Qed.
+
+  Lemma log_existsb_log_cons_neq :
+    forall (log: Log) idx idx' k p v f,
+      idx <> idx' ->
+      log_existsb (log_cons idx' (LE _ k p v) log) idx f =
+      log_existsb log idx f.
+  Proof.
+    unfold log_existsb; intros; rewrite log_cons_neq; eauto.
+  Qed.
+
+  Lemma log_existsb_empty :
+    forall idx f,
+      log_existsb (log_empty: Log) idx f = false.
+  Proof.
+    unfold log_existsb, log_empty; intros;
+      rewrite getenv_create; reflexivity.
+  Qed.
+
+  Lemma getenv_logapp:
+    forall (l l': Log) idx,
+      REnv.(getenv) (log_app l l') idx =
+      REnv.(getenv) l idx ++ REnv.(getenv) l' idx.
+  Proof.
+    unfold log_app, map2; intros; rewrite getenv_create; reflexivity.
+  Qed.
+
+  Lemma log_forallb_app:
+    forall (l l': Log) reg (f: LogEntryKind -> Port -> bool),
+      log_forallb (log_app l l') reg f =
+      log_forallb l reg f && log_forallb l' reg f.
+  Proof.
+    unfold log_forallb.
+    intros; rewrite getenv_logapp.
+    rewrite !forallb_app; reflexivity.
+  Qed.
+
+  Lemma log_existsb_app:
+    forall (l l': Log) reg (f: LogEntryKind -> Port -> bool),
+      log_existsb (log_app l l') reg f =
+      log_existsb l reg f || log_existsb l' reg f.
+  Proof.
+    unfold log_existsb, log_app; intros.
+    unfold map2; rewrite getenv_create.
+    rewrite existsb_app; reflexivity.
+  Qed.
+
+  Lemma log_app_assoc:
+    forall (l l' l'': Log),
+      log_app l (log_app l' l'') =
+      log_app (log_app l l') l''.
+  Proof.
+    unfold log_app, map2; intros.
+    apply create_funext; intros.
+    rewrite !getenv_create.
+    apply app_assoc.
+  Qed.
+
+  Lemma log_app_empty_l : forall (l: Log),
+      log_app l log_empty = l.
+  Proof.
+    intros.
+    apply equiv_eq.
+    unfold equiv, log_app, map2, log_empty; intros.
+    rewrite !getenv_create, app_nil_r.
+    reflexivity.
+  Qed.
+
+  Lemma log_app_empty_r : forall (l: Log),
+      log_app log_empty l = l.
+  Proof.
+    intros.
+    apply equiv_eq.
+    unfold equiv, log_app, map2, log_empty; intros.
+    rewrite !getenv_create.
+    reflexivity.
+  Qed.
 End Logs.
 
 Arguments LE {_}.
@@ -93,24 +235,38 @@ Section Interp.
 
   Notation Log := (Log R REnv).
 
+  Definition is_read0 kind prt :=
+    match kind, prt with
+    | LogRead, P0 => true
+    | _, _ => false
+    end.
+
+  Definition is_read1 kind prt :=
+    match kind, prt with
+    | LogRead, P1 => true
+    | _, _ => false
+    end.
+
+  Definition is_write0 kind prt :=
+    match kind, prt with
+    | LogWrite, P0 => true
+    | _, _ => false
+    end.
+
+  Definition is_write1 kind prt :=
+    match kind, prt with
+    | LogWrite, P1 => true
+    | _, _ => false
+    end.
+
+  Notation negf f := (fun kind prt => negb (f kind prt)).
+
   Definition may_read0 (sched_log rule_log: Log) idx :=
-    (log_forallb sched_log idx
-                 (fun kind prt => match kind, prt with
-                               | LogWrite, P0 => false
-                               | _, _ => true
-                               end)) &&
-    (log_forallb (log_app rule_log sched_log) idx
-                 (fun kind prt => match kind, prt with
-                               | LogWrite, P1 => false
-                               | _, _ => true
-                               end)).
+    negb (log_existsb sched_log idx is_write0) &&
+    negb (log_existsb (log_app rule_log sched_log) idx is_write1).
 
   Definition may_read1 (sched_log: Log) idx :=
-    log_forallb sched_log idx
-                (fun kind prt => match kind, prt with
-                              | LogWrite, P1 => false
-                              | _, _ => true
-                              end).
+    negb (log_existsb sched_log idx is_write1).
 
   Definition latest_write0 (log: Log) idx :=
     log_find log idx
@@ -119,18 +275,51 @@ Section Interp.
                      | _ => None
                      end).
 
+  Lemma latest_write0_empty idx:
+    latest_write0 (log_empty: Log) idx = None.
+  Proof.
+    apply log_find_empty.
+  Qed.
+
+  Lemma latest_write0_app :
+    forall (sl sl': Log) idx,
+      latest_write0 (log_app sl sl') idx =
+      match latest_write0 sl idx with
+      | Some e => Some e
+      | None => latest_write0 sl' idx
+      end.
+  Proof.
+    unfold latest_write0; eauto using log_find_app.
+  Qed.
+
+  Lemma latest_write0_cons_eq :
+    forall (log: Log) idx le,
+      latest_write0 (log_cons idx le log) idx =
+      match le with
+      | LE LogWrite P0 v => Some v
+      | _ => latest_write0 log idx
+      end.
+  Proof.
+    unfold latest_write0; intros.
+    rewrite log_find_cons_eq; destruct le, kind0, port0; reflexivity.
+  Qed.
+
+  Lemma latest_write0_cons_neq :
+    forall (log: Log) idx idx' le,
+      idx <> idx' ->
+      latest_write0 (log_cons idx' le log) idx =
+      latest_write0 log idx.
+  Proof.
+    unfold latest_write0; intros.
+    rewrite log_find_cons_neq by assumption; reflexivity.
+  Qed.
+
   Definition may_write (sched_log rule_log: Log) prt idx :=
     match prt with
-    | P0 => log_forallb (log_app rule_log sched_log) idx
-                       (fun kind prt => match kind, prt with
-                                     | LogRead, P1 | LogWrite, _ => false
-                                     | _, _ => true
-                                     end)
-    | P1 => log_forallb (log_app rule_log sched_log) idx
-                       (fun kind prt => match kind, prt with
-                                     | LogWrite, P1 => false
-                                     | _, _ => true
-                                     end)
+    | P0 => negb (log_existsb (log_app rule_log sched_log) idx is_read1) &&
+           negb (log_existsb (log_app rule_log sched_log) idx is_write0) &&
+           negb (log_existsb (log_app rule_log sched_log) idx is_write1)
+    | P1 => negb (log_existsb (log_app rule_log sched_log) idx is_write1)
     end.
 
   Notation expr := (expr var_t R Sigma).
@@ -225,3 +414,54 @@ Section Interp.
       interp_scheduler' log_empty s.
   End Scheduler.
 End Interp.
+
+
+Section EnvUpdates.
+  Context {reg_t: Type}.
+  Context {R: reg_t -> type}.
+  Context {REnv: Env reg_t}.
+
+  Definition rlog_latest_write_fn {k} (le: LogEntry (R k)) :=
+    match le with
+    | LE LogWrite _ v => Some v
+    | _ => None
+    end.
+
+  Definition latest_write (log: Log R REnv) idx :=
+    log_find log idx rlog_latest_write_fn.
+
+  Definition commit_update (r0: REnv.(env_t) R) (log: Log R REnv) : REnv.(env_t) R :=
+    REnv.(create) (fun k => match latest_write log k with
+                         | Some v => v
+                         | None => REnv.(getenv) r0 k
+                         end).
+
+  Lemma log_find_create {T}:
+    forall fn idx (f: LogEntry (R idx) -> option T),
+      log_find (REnv.(create) fn) idx f =
+      list_find_opt f (fn idx).
+  Proof.
+    unfold log_find; intros; rewrite getenv_create; reflexivity.
+  Qed.
+
+  Lemma commit_update_assoc:
+    forall (r : REnv.(env_t) R) (l l' : Log R REnv),
+      commit_update (commit_update r l) l' = commit_update r (log_app l' l).
+  Proof.
+    unfold commit_update, log_app, map2, latest_write, log_find; intros.
+    apply create_funext; intros.
+    rewrite !getenv_create.
+    rewrite list_find_opt_app.
+    destruct list_find_opt; reflexivity.
+  Qed.
+
+  Lemma commit_update_empty:
+    forall (r : REnv.(env_t) R),
+      commit_update r log_empty = r.
+  Proof.
+    intros; apply equiv_eq; intro.
+    unfold commit_update, log_empty, latest_write, log_find; rewrite !getenv_create.
+    reflexivity.
+  Qed.
+End EnvUpdates.
+
